graph/spanning_tree.v
@@ -1395,10 +1395,10 @@ Section SPANNING.
   Context {V E: Type}.
   Context {EV: EqDec V eq}.
   Context {EE: EqDec E eq}.
-  Context {DV DE: Type}.
+  Context {DV DE DG: Type}.
   Context {MGS: MarkGraphSetting DV}.
-  Context {P: LabeledGraph V E DV DE -> Type}.
-  Notation Graph := (GeneralGraph V E DV DE P).
+  Context {P: LabeledGraph V E DV DE DG -> Type}.
+  Notation Graph := (GeneralGraph V E DV DE DG P).
   Local Coercion pg_lg : LabeledGraph >-> PreGraph.
   Local Coercion lg_gg : GeneralGraph >-> LabeledGraph.
 
