graph/weak_mark_lemmas.v
@@ -54,10 +54,10 @@ Section WeakMarkGraph.
 Context {V E: Type}.
 Context {EV: EqDec V eq}.
 Context {EE: EqDec E eq}.
-Context {DV DE: Type}.
+Context {DV DE DG: Type}.
 Context {MGS: MarkGraphSetting DV}.
 
-Notation Graph := (LabeledGraph V E DV DE).
+Notation Graph := (LabeledGraph V E DV DE DG).
 Local Coercion pg_lg : LabeledGraph >-> PreGraph.
 
 Definition marked (g: Graph) : NodePred V.
